cleanq/rb: new weak frame condition for the model based on the RB frame conditions
Signed-off-by: Roni Häcki <roni.haecki@inf.ethz.ch>

CleanQ/CleanQ_RBModel.thy
@@ -211,45 +211,36 @@ subsubsection \<open>Strong and Weak frame condition\<close>
 text \<open>The strong frame condition fixed the full state except for the part which should
       change. \<close>
 definition frame_rb_strong :: "'a CleanQ_RB_State \<Rightarrow> 'a CleanQ_RB_State \<Rightarrow> bool"
-  where "frame_rb_strong rb' rb \<longleftrightarrow> rb' = rb"
+  where "frame_rb_strong rb' rb \<longleftrightarrow> rb' = rb \<and> I4_rb_valid rb"
 
 text \<open>
   Assuming a two concurrently acting agents, we can not assume that all of the RB state
   stays the same. In order to model this, we have to weaken the frame condition which
   we up to now implicitly used. \<close>
-(* Need to express somehow that descriptors can be added by enq *)
 definition frame_rb_weak_x :: "'a CleanQ_RB_State \<Rightarrow> 'a CleanQ_RB_State \<Rightarrow> bool"
-  where "frame_rb_weak_x st' st \<longleftrightarrow>
-   (\<exists>\<delta>tyx \<delta>txy.
-    ring (rTXY st') = ring (rTXY st) \<and>
-    size (rTXY st') = size (rTXY st) \<and>
-    size (rTYX st') = size (rTYX st) \<and>
-    rSX st' = rSX st \<and>
-    CleanQ_RB_list (rTXY st') =  CleanQ_RB_list (rTXY st) @ \<delta>tyx \<and>
-    \<delta>tyx @ CleanQ_RB_list (rTYX st') = CleanQ_RB_list (rTYX st) \<and>
-    rSY st' = \<delta>txy \<union> rSY st - (set \<delta>tyx))" 
+  where "frame_rb_weak_x st' st \<longleftrightarrow> rSX st = rSX st' \<and> frame_rb_weak_left (rTXY st') (rTXY st) 
+                                    \<and> frame_rb_weak_right (rTYX st') (rTYX st) \<and>
+                                    (\<exists>\<delta>txy \<delta>tyx. rSY st' = \<delta>txy \<union> rSY st - (set \<delta>tyx))" 
 
 definition frame_rb_weak_y :: "'a CleanQ_RB_State \<Rightarrow> 'a CleanQ_RB_State \<Rightarrow> bool"
-  where "frame_rb_weak_y st' st \<longleftrightarrow>
-    head (rTYX st') = head (rTYX st) \<and>
-    tail (rTXY st') = tail (rTXY st) \<and>
-    ring (rTYX st') = ring (rTYX st) \<and>
-    size (rTYX st') = size (rTYX st) \<and>
-    size (rTXY st') = size (rTXY st) \<and>
-    rSY st' = rSY st \<and>
-    (\<exists>\<delta>hd \<delta>tl \<delta>dc.
-        tail (rTYX st') + \<delta>tl = tail (rTYX st)\<and>
-        head (rTXY st') + \<delta>hd = head (rTXY st)\<and>
-        CleanQ_RB_list (rTXY st') =  \<delta>dc @ CleanQ_RB_list (rTXY st))" (*X adding something to ring*)
+  where "frame_rb_weak_y st' st \<longleftrightarrow> rSY st = rSY st' \<and> frame_rb_weak_left (rTYX st') (rTYX st) \<and>
+                                    frame_rb_weak_right (rTXY st') (rTXY st) \<and>
+                                    (\<exists>\<delta>txy \<delta>tyx. rSX st' = \<delta>tyx \<union> rSX st - (set \<delta>txy))"
 
 lemma frame_rb_s_w_x:
-  "frame_rb_strong dev' dev \<Longrightarrow> frame_rb_weak_x dev' dev"
-  by (smt Diff_empty Un_commute append_Nil2 frame_rb_strong_def 
-      frame_rb_weak_x_def list.set(1) self_append_conv2 sup_bot.comm_neutral)
+ "frame_rb_strong st' st \<Longrightarrow> frame_rb_weak_x st' st"
+  unfolding frame_rb_weak_x_def frame_rb_strong_def frame_rb_weak_left_def
+  frame_rb_weak_right_def
+  by (metis Diff_empty I4_rb_valid.elims(2) Un_absorb add.commute add.left_neutral list.set(1) 
+      rb_valid_def rb_valid_ptr_def)
+ 
 
 lemma frame_rb_s_w_y:
   "frame_rb_strong dev' dev \<Longrightarrow> frame_rb_weak_y dev' dev"
-  by(simp add:frame_rb_strong_def frame_rb_weak_y_def)
+  unfolding frame_rb_weak_y_def frame_rb_strong_def frame_rb_weak_left_def
+  frame_rb_weak_right_def
+  by (metis Diff_empty I4_rb_valid.elims(2) Un_absorb add.commute add.left_neutral list.set(1) 
+      rb_valid_def rb_valid_ptr_def)
 
 (* ------------------------------------------------------------------------------------ *)
 subsubsection \<open>All CleanQ RB Invariants\<close>
@@ -281,32 +272,22 @@ lemma frame_rb_weak_x_list_weak:
   fixes rb rb' K
   assumes I1: "CleanQ_RB_Invariants K rb'"
       and frame: "frame_rb_weak_x rb' rb"
-    shows "frame_list_weak (lTXY (CLeanQ_RB2List rb'), lSY (CleanQ_RB2List rb'), lTYX (CleanQ_RB2List rb'), lSX (CleanQ_RB2List rb')) 
-                           (lTXY (CLeanQ_RB2List rb), lSY (CleanQ_RB2List rb), lTYX (CleanQ_RB2List rb), lSX (CleanQ_RB2List rb))"
-  unfolding CleanQ_RB2List_def
-proof auto
+    shows "frame_list_weak (lTXY (CleanQ_RB2List rb'), lSY (CleanQ_RB2List rb'), lTYX (CleanQ_RB2List rb'), lSX (CleanQ_RB2List rb')) 
+                           (lTXY (CleanQ_RB2List rb), lSY (CleanQ_RB2List rb), lTYX (CleanQ_RB2List rb), lSX (CleanQ_RB2List rb))"
+  unfolding CleanQ_RB2List_def CleanQ_RB_list_def
+  apply auto 
+proof -
+  show "\<And>x. x \<in> rSX rb' \<Longrightarrow> x \<in> rSX rb"
+    by (metis frame frame_rb_weak_x_def) 
+  show " \<And>x. x \<in> rSX rb \<Longrightarrow> x \<in> rSX rb'"
+    by (metis frame frame_rb_weak_x_def)
 
-  show "\<And>x. x \<in> rSX rb' \<Longrightarrow> x \<in> rSX rb" using frame by (simp add: frame_rb_weak_x_def)
-  show "\<And>x. x \<in> rSX rb \<Longrightarrow> x \<in> rSX rb'" using frame by (simp add: frame_rb_weak_x_def)
-
-    from frame obtain \<delta>hd \<delta>tl where
-    dHd: "head (rTXY rb') + \<delta>hd = head (rTXY rb)" and
-    dTl: "tail (rTYX rb') + \<delta>tl = tail (rTYX rb)"
-      by (simp add: frame_rb_weak_x_def)
-
-
-  define \<delta>txy where "\<delta>txy =  map (ring (rTXY rb')) \<delta>hd"
-  define \<delta>bc where "\<delta>bc = slice (BF dev') (dn dev') (dn dev)"
-  (* Somehow this does not seem to work
-    from frame obtain \<delta>dc where
-    dDc: "CleanQ_RB_list (rTXY rb') = \<delta>dc @ CleanQ_RB_list (rTXY rb)"  
-      unfolding CleanQ_RB_list_def
-  *)
-    
+  have "rb_valid_entries (rTXY rb') = (rb_delta_tail n (rTXY rb)) @ (rb_valid_entries (rTXY rb))"
+    using rb_weak_delta_tail_n
 
 
 qed
-*) 
+*)
 (* ==================================================================================== *)
 subsection \<open>State Transition Operations\<close>
 (* ==================================================================================== *)
